generational/spec/GC.Gen.ChunkedCheney.fst
@@ -359,6 +359,22 @@ let chunked_cheney_promote_equation
            fwd_map = cs2.ccs_fwd }))
   = ()
 
+let chunked_cheney_collect_spec_equation
+  (minor: minor_state) (major: MH.major_heap) (fp: U64.t)
+  (roots: seq U64.t) (alloc_fuel: nat)
+  : Lemma
+      (ensures
+        (let prom = chunked_cheney_promote minor major fp roots alloc_fuel in
+         chunked_cheney_collect_spec minor major fp roots alloc_fuel ==
+         { cmc_major =
+            ChunkedUpdate.chunked_update_major_pointers
+              prom.major_final prom.fwd_map;
+           cmc_fp    = prom.fp_final;
+           cmc_minor = minor_reset minor;
+           cmc_roots = rewrite_roots roots prom.fwd_map;
+           cmc_fwd   = prom.fwd_map }))
+  = ()
+
 #push-options "--z3rlimit 5 --fuel 0 --ifuel 0 --split_queries always"
 let chunked_cheney_forward_normal_default_single_chunk_compat
   (minor: minor_state) (cs: Dense.cheney_state) (addr: U64.t)
